\documentclass[12pt]{article}

\usepackage{amsmath}
\usepackage{amssymb}
\usepackage{ascmac}
\usepackage[all]{xy}
\usepackage{ebproof}

\setlength{\paperwidth}{20cm}
\setlength{\paperheight}{20cm}

\input{layout.tex}

\begin{document}
\pagestyle{empty}

\[
  \begin{prooftree}
    \infer0{\langle \epsilon, x\rangle \to \mathbf{s}(\epsilon)}
  \end{prooftree}
\]

\[
  \begin{prooftree}
    \infer0{\langle \sigma,\sigma x\rangle \to \mathbf{s}(\sigma)}
  \end{prooftree}
  \quad
  \begin{prooftree}
    \hypo{\sigma \neq \sigma'}
    \infer1{\langle \sigma,\sigma' x\rangle \to \mathbf{f}}
  \end{prooftree}
\]

\[
  \begin{prooftree}
    \hypo{A \leftarrow e \in R}
    \hypo{\langle e, x\rangle \to o}
    \infer2{\langle A, x\rangle \to o}
  \end{prooftree}
\]

\[
  \begin{prooftree}
    \hypo{\langle e_1,x_1x_2y\rangle\to \mathbf{s}(x_1)}
    \hypo{\langle e_2, x_2y\rangle \to \mathbf{s}(x_2)}
    \infer2{\langle e_1e_2, x_1x_2y\rangle \to \mathbf{s}(x_1x_2)}
  \end{prooftree}
  \quad
  \begin{prooftree}
    \hypo{\langle e_1,x\rangle \to \mathbf{f}}
    \infer1{\langle e_1e_2, x\rangle \to \mathbf{f}}
  \end{prooftree}
  \quad
  \begin{prooftree}
    \hypo{\langle e_1,x_1y\rangle\to \mathbf{s}(x_1)}
    \hypo{\langle e_2, y\rangle \to \mathbf{f}}
    \infer2{\langle e_1e_2, x_1y\rangle \to \mathbf{f}}
  \end{prooftree}
\]

\[
  \begin{prooftree}
    \hypo{\langle e_1,xy\rangle \to \mathbf{s}(x)}
    \infer1{\langle e_1 / e_2,xy\rangle \to \mathbf{s}(x)}
  \end{prooftree}
  \quad
  \begin{prooftree}
    \hypo{\langle e_1,x\rangle \to \mathbf{f}}
    \hypo{\langle e_2,x\rangle \to o}
    \infer2{\langle e_1 / e_2,x\rangle \to o}
  \end{prooftree}
\]

\[
  \begin{prooftree}
    \hypo{\langle e,x_1x_2y\rangle \to \mathbf{s}(x_1)}
    \hypo{\langle e^*,x_2y\rangle \to \mathbf{s}(x_2)}
    \infer2{\langle e^*,x_1x_2y\rangle \to \mathbf{s}(x_1x_2)}
  \end{prooftree}
  \quad
  \begin{prooftree}
    \hypo{\langle e,x\rangle \to \mathbf{f}}
    \infer1{\langle e^*,x\rangle \to \mathbf{s}(\epsilon)}
  \end{prooftree}
\]

\[
  \begin{prooftree}
    \hypo{\langle e,x\rangle \to \mathbf{f}}
    \infer1{\langle !e, x\rangle \to \mathbf{s}(\epsilon)}
  \end{prooftree}
  \quad
  \begin{prooftree}
    \hypo{\langle e,xy\rangle \to \mathbf{s}(x)}
    \infer1{\langle !e,xy\rangle \to \mathbf{f}}
  \end{prooftree}
\]

\[
  \begin{prooftree}
    \hypo{\langle e\; e^*,x\rangle \to o}
    \infer1{\langle e+,x\rangle \to o}
  \end{prooftree}
  \quad
  \begin{prooftree}
    \hypo{\langle e / \epsilon,x\rangle \to o}
    \infer1{\langle e?,x\rangle \to o}
  \end{prooftree}
  \quad
  \begin{prooftree}
    \hypo{\langle !!e,x\rangle \to o}
    \infer1{\langle \& e,x\rangle \to o}
  \end{prooftree}
\]

\end{document}
