\documentclass[12pt]{article}

\usepackage{amsmath}
\usepackage{amssymb}
\usepackage{ascmac}
\usepackage{mathtools}
\usepackage{ebproof}

\setlength{\paperwidth}{100cm}
\setlength{\paperheight}{30cm}

\input{layout.tex}

\begin{document}
\pagestyle{empty}

\[
    \begin{prooftree}
        \infer0{\mathbf{fresh} \beta_1}
        \infer0{\mathcal{W}_{\text{simply}}(\mathit{id}: \beta_1, \mathit{id}) = (\emptyset, \beta_1)}
        \infer0{\mathbf{fresh} \beta_2}
        \infer0{\mathcal{W}_{\text{simply}}(\mathit{id}: \beta_1, x: \beta_2, x) = (\emptyset, \beta_2)}
        \infer2{\mathcal{W}_{\text{simply}}(\mathit{id}: \beta_1, \lambda x\ldotp x) = (\emptyset, \beta_2 \to \beta_2)}
        \infer0{\mathbf{fresh} \beta_3}
        \infer0{\mathcal{U}(\beta_1, (\beta_2 \to \beta_2) \to \beta_3) = S_1}
        \infer4{\mathcal{W}_{\text{simply}}(\mathit{id}: \beta_1, \mathit{id}\;(\lambda x\ldotp x)) = (S_1 = \{\beta_1 \mapsto (\beta_2 \to \beta_2) \to \beta_3\}, \beta_3)}
        \infer0{\mathcal{W}_{\text{simply}}(\mathit{id}: (\beta_2 \to \beta_2) \to \beta_3, \mathit{id}) = (\emptyset, (\beta_2 \to \beta_2) \to \beta_3)}
        \infer0{\mathcal{W}_{\text{simply}}(\mathit{id}: (\beta_2 \to \beta_2) \to \beta_3, \text{\texttt{()}}) = (\emptyset, \mathbf{unit})}
        \infer0{\mathbf{fresh} \beta_4}
        \hypo{\mathcal{U}((\beta_2 \to \beta_2) \to \beta_3, \mathbf{unit} \to \beta_4) = S_2}
        \infer4{\mathcal{W}_{\text{simply}}(\mathit{id}: (\beta_2 \to \beta_2) \to \beta_3, \mathit{id}\;\text{\texttt{()}}) = (S_2, ?)}
        \infer0{\mathbf{fresh} \beta_5}
        \hypo{\mathcal{U}(\beta_3, ? \to \beta_5) = S_3}
        \infer4{\mathcal{W}_{\text{simply}}(\mathit{id}: \beta_1, (\mathit{id}\;(\lambda x\ldotp x))\;(\mathit{id}\;\text{\texttt{()}})) = (S_3S_2S_1, ?)}
        \infer2{\mathcal{W}_{\text{simply}}(\emptyset, \lambda \mathit{id}\ldotp (\mathit{id}\;(\lambda x\ldotp x))\;(\mathit{id}\;\text{\texttt{()}})) = (S_3S_2S_1, ?)}
    \end{prooftree}
\]
\end{document}
