\documentclass[12pt]{article}

\usepackage{amsmath}
\usepackage{amssymb}
\usepackage{ascmac}
\usepackage{mathtools}
\usepackage{ebproof}

\setlength{\paperwidth}{20cm}
\setlength{\paperheight}{30cm}

\input{layout.tex}

\begin{document}
\pagestyle{empty}

\begin{align*}
    \tau &\Coloneqq \alpha \mid \mathbf{unit} \mid \tau \to \tau \\
    \mathbf{default}(\tau) &= \left\{\begin{array}{ll}
        \mathbf{unit} &(\tau = \alpha \lor \tau = \mathbf{unit}) \\
        \mathbf{default}(\tau_1) \to \mathbf{default}(\tau_2) &(\tau = \tau_1 \to \tau_2)
    \end{array}\right.
\end{align*}

\[
    \begin{prooftree}
        \infer0{\mathcal{W}_{\text{simply}}(\Gamma, \text{\texttt{()}}) = (\emptyset, \mathbf{unit})}
    \end{prooftree}
\]

\[
    \begin{prooftree}
        \infer0{\mathcal{W}_{\text{simply}}(\Gamma, x) = (\emptyset, \Gamma(x))}
    \end{prooftree}
\]

\[
    \begin{prooftree}
        \hypo{\mathbf{fresh} \beta}
        \hypo{\mathcal{W}_{\text{simply}}(\Gamma + x:\beta, e) = (S_1, \tau_1)}
        \infer2{\mathcal{W}_{\text{simply}}(\Gamma, \lambda x\ldotp e) = (S_1, S_1\beta \to \tau_1)}
    \end{prooftree}
\]

\[
    \begin{prooftree}
        \hypo{\mathcal{W}_{\text{simply}}(\Gamma, e_1) = (S_1, \tau_1)}
        \hypo{\mathcal{W}_{\text{simply}}(S_1\Gamma, e_2) = (S_2, \tau_2)}
        \hypo{\mathbf{fresh} \beta}
        \hypo{\mathcal{U}(S_2\tau_1, \tau_2 \to \beta) = S_3}
        \infer4{\mathcal{W}_{\text{simply}}(\Gamma, e_1\; e_2) = (S_3S_2S_1, S_3\beta)}
    \end{prooftree}
\]
\end{document}
