\documentclass[12pt]{article}

\usepackage{amsmath}
\usepackage{amssymb}
\usepackage{ascmac}
\usepackage{mathtools}
\usepackage{ebproof}

\setlength{\paperwidth}{20cm}
\setlength{\paperheight}{30cm}

\input{layout.tex}

\begin{document}
\pagestyle{empty}

\[
    \begin{prooftree}
        \hypo{\mathcal{U}(\rho, \mathbf{unit}) = S}
        \infer1{\mathcal{M}(\Gamma, \text{\texttt{()}}, \rho) = S}
    \end{prooftree}
\]

\[
    \begin{prooftree}
        \hypo{\Gamma(x) = \forall \vec{\alpha}\ldotp \tau}
        \hypo{\mathbf{fresh} \vec{\beta}}
        \hypo{\mathcal{U}(\rho, \tau[\vec{\alpha} \leftarrow \vec{\beta}]) = S}
        \infer3{\mathcal{M}(\Gamma, x, \rho) = S}
    \end{prooftree}
\]

\[
    \begin{prooftree}
        \hypo{\mathbf{fresh} \beta_1, \beta_2}
        \hypo{\mathcal{U}(\rho, \beta_1 \to \beta_2) = S_1}
        \hypo{\mathcal{M}(S_1\Gamma + x:S_1\beta_1, e, S_1\beta_2) = S_2}
        \infer3{\mathcal{W}(\Gamma, \lambda x\ldotp e, \rho) = S_2S_1}
    \end{prooftree}
\]

\[
    \begin{prooftree}
        \hypo{\mathbf{fresh} \beta}
        \hypo{\mathcal{M}(\Gamma, e_1, \beta \to \rho) = S_1}
        \hypo{\mathcal{M}(S_1\Gamma, e_2, S_1\beta) = S_2}
        \infer3{\mathcal{M}(\Gamma, e_1\; e_2, \rho) = S_2S_1}
    \end{prooftree}
\]

\[
    \begin{prooftree}
        \hypo{\mathbf{fresh} \beta}
        \hypo{\mathcal{M}(\Gamma, e_1, \beta) = S_1}
        \hypo{\Gamma_1 = S_1(\Gamma)}
        \hypo{\mathcal{M}(\Gamma_1 + x:\mathrm{Gen}(\Gamma_1, S_1\beta), e_2, S_1\rho) = S_2}
        \infer4{\mathcal{M}(\Gamma, \mathbf{let}\;x = e_1\;\mathbf{in}\; e_2, \rho) = S_2S_1}
    \end{prooftree}
\]
\end{document}
