\documentclass[12pt]{article}

\usepackage{amsmath}
\usepackage{amssymb}
\usepackage[all]{xy}
\usepackage{ebproof}

\setlength{\paperwidth}{10cm}
\setlength{\paperheight}{30cm}

\input{layout.tex}

\begin{document}
\pagestyle{empty}

\[
  \begin{prooftree}
    \hypo{A \in \mathcal{A}}
    \infer1[type]{\vdash \mathop{\mathbf{type}} A}
  \end{prooftree}
\]

\[
  \begin{prooftree}
    \hypo{E \in \mathcal{E}}
    \infer1[effect]{\vdash \mathop{\mathbf{effect}} E}
  \end{prooftree}
\]

\[
  \begin{prooftree}
    \hypo{\vdash \mathop{\mathbf{effect}} \epsilon}
    \hypo{\vdash \mathop{\mathbf{type}} \tau}
    \infer2[type lift]{\vdash \mathop{\mathbf{type}} T \epsilon \tau}
  \end{prooftree}
\]

\[
  \begin{prooftree}
    \hypo{\vdash \mathop{\mathbf{type}} \tau}
    \infer1[var]{x: \tau \vdash x: \tau}
  \end{prooftree}
\]

\[
  \begin{prooftree}
    \hypo{x: \tau_1 \vdash e: \tau_2}
    \infer1[lift]{x: \tau_1 \vdash [e]: T 1 \tau_2}
  \end{prooftree}
\]

\[
  \begin{prooftree}
    \hypo{x: \tau \vdash e: \tau_1}
    \hypo{f: \tau_1 \to \tau_2 \in \mathcal{F}}
    \infer2[app]{x: \tau \vdash f(e): \tau_2}
  \end{prooftree}
\]

\[
  \begin{prooftree}
    \hypo{x: \tau \vdash e: \tau_1}
    \hypo{f: \tau_1 \xrightarrow{\epsilon} \tau_2 \in \mathcal{F}}
    \infer2[effectful app]{x: \tau \vdash f(e): T \epsilon \tau_2}
  \end{prooftree}
\]

\[
  \begin{prooftree}
    \hypo{x: \tau_1 \vdash e_1: T \epsilon_1 \tau_2}
    \hypo{x_1: \tau_2 \vdash e_2: T \epsilon_2 \tau_3}
    \infer2[let]{x: \tau_1 \vdash (\mathop{\mathbf{let}} x_1 \gets e_1 \mathop{\mathbf{in}} e_2): T (\epsilon_1 \cdot \epsilon_2) \tau_3}
  \end{prooftree}
\]

\[
  \begin{prooftree}
    \hypo{\vdash \mathop{\mathbf{effect}} \epsilon_1}
    \hypo{\vdash \mathop{\mathbf{effect}} \epsilon_2}
    \infer2[effect ord]{\vdash \epsilon_1 \sqsubseteq \epsilon_2}
  \end{prooftree}
\]

\[
  \begin{prooftree}
    \hypo{x: \tau_1 \vdash e: T \epsilon_1 \tau_2}
    \hypo{\vdash \epsilon_1 \sqsubseteq \epsilon_2}
    \infer2[cast]{x: \tau_1 \vdash e: T \epsilon_2 \tau_2}
  \end{prooftree}
\]

\[
  \begin{prooftree}
    \hypo{x: \tau_1 \vdash e_1: \tau_2}
    \hypo{x: \tau_1 \vdash e_2: \tau_2}
    \infer2[eq]{x: \tau_1 \vdash e_1 =_{\tau_2} e_2}
  \end{prooftree}
\]
\end{document}
